Translation/PackLifts.v
@@ -32,6 +32,7 @@ Fixpoint llift γ δ (t:sterm)  : sterm :=
   | sApp u A B v =>
     sApp (llift γ δ u) (llift γ δ A) (llift γ (S δ) B) (llift γ δ v)
   | sProd na A B => sProd na (llift γ δ A) (llift γ (S δ) B)
+  | sSum na A B => sSum na (llift γ δ A) (llift γ (S δ) B)
   | sEq A u v => sEq (llift γ δ A) (llift γ δ u) (llift γ δ v)
   | sRefl A u => sRefl (llift γ δ A) (llift γ δ u)
   | sJ A u P w v p =>
@@ -86,6 +87,7 @@ Fixpoint rlift γ δ t : sterm :=
   | sApp u A B v =>
     sApp (rlift γ δ u) (rlift γ δ A) (rlift γ (S δ) B) (rlift γ δ v)
   | sProd na A B => sProd na (rlift γ δ A) (rlift γ (S δ) B)
+  | sSum na A B => sSum na (rlift γ δ A) (rlift γ (S δ) B)
   | sEq A u v => sEq (rlift γ δ A) (rlift γ δ u) (rlift γ δ v)
   | sRefl A u => sRefl (rlift γ δ A) (rlift γ δ u)
   | sJ A u P w v p =>
@@ -1022,6 +1024,7 @@ Proof.
         rewrite llift_subst. cbn.
         replace (#|Δ| + 0)%nat with #|Δ| by omega.
         eapply type_App ; emh.
+      - cbn. eapply type_Sum ; emh.
       - cbn. eapply type_Eq ; emh.
       - cbn. eapply type_Refl ; emh.
       - cbn. replace #|Δ| with (#|Δ| + 0)%nat by omega.
@@ -1144,6 +1147,7 @@ Proof.
         rewrite rlift_subst. cbn.
         replace (#|Δ| + 0)%nat with #|Δ| by omega.
         eapply type_App ; emh.
+      - cbn. eapply type_Sum ; emh.
       - cbn. eapply type_Eq ; emh.
       - cbn. eapply type_Refl ; emh.
       - cbn. replace #|Δ| with (#|Δ| + 0)%nat by omega.
