Translation/Uniqueness.v
@@ -33,6 +33,12 @@ Proof.
     pose proof (sort_conv_inv IHu2) as e2.
     subst. apply conv_refl.
   - eapply nl_conv ; try eassumption ; reflexivity.
+  - specialize (IHu1 _ _ _ h h0).
+    specialize (IHu2 _ _ _ h4 h7).
+    eapply conv_trans ; try eapply h6.
+    pose proof (sort_conv_inv IHu1) as e1.
+    pose proof (sort_conv_inv IHu2) as e2.
+    subst. apply conv_refl.
   - specialize (IHu1 _ _ _ h0 h6).
     pose proof (sort_conv_inv IHu1) as e. subst. assumption.
   - specialize (IHu1 _ _ _ h h0).
